Flapjack/Test/AllocatorCore.lean
@@ -47,6 +47,34 @@ example :
   exact wordProgClashAnalysis_ite
 
 example :
+    (2, 4) ∈ (wordProgClashAnalysis
+      ((.call none none []
+        (some (9, (.assign 2 (.var 3) : WordProg Nat)))) : WordProg Nat)
+      [4]).2 := by
+  native_decide
+
+example :
+    (9, 3) ∈ (wordProgClashAnalysis
+      ((.call none none []
+        (some (9, (.assign 2 (.var 3) : WordProg Nat)))) : WordProg Nat)
+      [4]).2 := by
+  native_decide
+
+example :
+    9 ∈ (wordProgClashAnalysis
+      ((.call none none []
+        (some (9, (.assign 2 (.var 3) : WordProg Nat)))) : WordProg Nat)
+      [4]).1 := by
+  native_decide
+
+example :
+    3 ∈ (wordProgClashAnalysis
+      ((.call none none []
+        (some (9, (.assign 2 (.var 3) : WordProg Nat)))) : WordProg Nat)
+      [4]).1 := by
+  native_decide
+
+example :
     (wordAllocateSsaProgram
       ({ current := [], next := 10 } : WordSsaState)
       ((.ite .equal 0 (.reg 0)
